vale/code/arch/x64/Vale.X64.Memory.fst
@@ -724,8 +724,9 @@ let inv_buffer_info (bi:buffer_info) (owners:heaplet_id -> Set.set int) (h:vale_
 let inv_heaplets (layout:vale_heap_layout_inner) (h:vale_heap) (hs:vale_heaplets) (mt:memTaint_t) =
   let bs = layout.vl_buffers in
   modifies layout.vl_mod_loc layout.vl_old_heap h /\  // modifies for entire heap
-  (forall (i:heaplet_id) (a:int).{:pattern Set.mem a (layout.vl_heaplet_sets i)}
-    layout.vl_heaplet_map a == Some i <==> Set.mem a (layout.vl_heaplet_sets i)
+  (forall (i:heaplet_id).{:pattern layout.vl_heaplet_sets i}
+    forall (a:int).{:pattern Set.mem a (layout.vl_heaplet_sets i) \/ layout.vl_heaplet_map a}
+      layout.vl_heaplet_map a == Some i <==> Set.mem a (layout.vl_heaplet_sets i)
   ) /\
   (forall (i:heaplet_id).{:pattern (Map16.sel hs i)}
     inv_heaplet (layout.vl_heaplet_sets i) h (Map16.sel hs i)) /\
@@ -735,12 +736,19 @@ let inv_heaplets (layout:vale_heap_layout_inner) (h:vale_heap) (hs:vale_heaplets
     i1 < Seq.length bs /\ i2 < Seq.length bs ==> buffer_info_disjoint (Seq.index bs i1) (Seq.index bs i2)) /\
   True
 
-let is_initial_heap layout h =
+let is_initial_heap_def layout h =
   h == layout.vl_inner.vl_old_heap /\
   not layout.vl_inner.vl_heaplets_initialized
 
 let mem_inv h =
   h.vf_heap.heapletId == None /\
+  ( match h.vf_layout.vl_heaplet_domains with
+    | None -> True
+    | Some d ->
+      (forall (i:int).{:pattern d i \/ h.vf_layout.vl_inner.vl_heaplet_map i}
+        let k = h.vf_layout.vl_inner.vl_heaplet_map i in
+        Some? k ==> d i == k)
+  ) /\
   inv_heaplet_ids h.vf_heaplets /\
   (if h.vf_layout.vl_inner.vl_heaplets_initialized
     then
