vale/specs/hardware/Vale.Arch.HeapTypes_s.fst
@@ -1,5 +1,6 @@
 module Vale.Arch.HeapTypes_s
 open FStar.Mul
+open Vale.Def.Words_s
 
 let __reduce__ = ()
 
@@ -14,6 +15,22 @@ type taint:eqtype =
   | Public
   | Secret
 
-type memTaint_t = (m:Map.t int taint{Set.equal (Map.domain m) (Set.complement Set.empty)})
-
+let machine_heap = Map.t int nat8
+let memTaint_t = (m:Map.t int taint{Set.equal (Map.domain m) (Set.complement Set.empty)})
 let heaplet_id = n:nat{n < 16}
+
+let heaplets8 (ptr:int) (k:heaplet_id) (m:option (int -> option heaplet_id)) : bool =
+  match m with None -> true | Some d -> d ptr = Some k
+
+let heaplets16 (ptr:int) (k:heaplet_id) (m:option (int -> option heaplet_id)) : bool =
+  heaplets8 ptr k m && heaplets8 (ptr + 1) k m 
+
+let heaplets32 (ptr:int) (k:heaplet_id) (m:option (int -> option heaplet_id)) : bool =
+  heaplets16 ptr k m && heaplets16 (ptr + 2) k m 
+
+[@"opaque_to_smt"]
+let heaplets64 (ptr:int) (k:heaplet_id) (m:option (int -> option heaplet_id)) : bool =
+  heaplets32 ptr k m && heaplets32 (ptr + 4) k m 
+
+let heaplets128 (ptr:int) (k:heaplet_id) (m:option (int -> option heaplet_id)) : bool =
+  heaplets64 ptr k m && heaplets64 (ptr + 8) k m 
